theories/datatypes_properties.v
@@ -311,11 +311,15 @@ Definition administrative_instruction_ind' (P : administrative_instruction -> Pr
 
 (** Administrative instructions frequently come in lists.
   Here is the corresponding induction principle. **)
+(* TODO: rect'_build_list fails to generate wellformed definitions on newer versions
+   of Coq. Use manual versions for now *)
+(*
 Definition seq_administrative_instruction_rect' :=
   ltac:(rect'_build_list administrative_instruction_rect).
 
 Definition seq_administrative_instruction_ind' (P : administrative_instruction -> Prop) :=
   @seq_administrative_instruction_rect' P.
+*)
 
 Definition administrative_instruction_eq_dec : forall e1 e2 : administrative_instruction,
   {e1 = e2} + {e1 <> e2}.
